src/CoopConcurMonad.v
@@ -1,0 +1,86 @@
+Require Import CoopConcur.
+
+Ltac inv_step :=
+  match goal with
+  | [ H: step _ _ _ _ _ |- _ ] =>
+    inversion H;
+    subst;
+    repeat sigT_eq;
+    subst
+  end.
+
+Ltac inv_fail_step :=
+  match goal with
+  | [ H: fail_step _ _ _ _ |- _ ] =>
+    inversion H;
+    subst;
+    repeat sigT_eq;
+    subst
+  end.
+
+Ltac inv_exec' H :=
+  inversion H; subst;
+  repeat sigT_eq;
+  try inv_step;
+  try inv_fail_step.
+
+Ltac inv_exec :=
+  lazymatch goal with
+  | [ H: exec _ _ (Ret _) _ _ |- _ ] =>
+    inv_exec' H
+  | [ H: exec _ _ (Bind _ _) _ _ |- _ ] =>
+    inv_exec' H
+  | [ H: exec _ _ _ _ _ |- _ ] =>
+    inv_exec' H
+  end.
+
+Section MonadLaws.
+  Hint Constructors step exec.
+
+  Infix "~=" := prog_equiv (at level 50, left associativity).
+
+  Theorem bind_left_id : forall T T' Sigma v (p: T -> prog Sigma T'),
+      Bind (Ret v) p ~= p v.
+  Proof.
+    split; intros.
+    - inv_exec.
+      inv_exec; eauto.
+      inv_exec; eauto.
+    - eauto.
+  Qed.
+
+  Theorem bind_right_id : forall T Sigma (p: prog Sigma T),
+      Bind p Ret ~= p.
+  Proof.
+    split; intros.
+    - inv_exec; eauto.
+      inv_exec; eauto.
+    - destruct out; eauto.
+  Qed.
+
+  Theorem bind_assoc : forall Sigma T T' T'' (p1: prog Sigma T) (p2: T -> prog Sigma T') (p3: T' -> prog Sigma T''),
+      Bind (Bind p1 p2) p3 ~= Bind p1 (fun x => Bind (p2 x) p3).
+  Proof.
+    split; intros.
+    - inv_exec; eauto;
+        inv_exec; eauto.
+    - inv_exec; eauto.
+      inv_exec; eauto.
+  Qed.
+
+End MonadLaws.
+
+Ltac monad_simpl_one :=
+  match goal with
+  | [ |- valid _ _ _ (Bind (Ret _) _) ] =>
+    eapply valid_equiv;
+    [ apply bind_left_id | ]
+  | [ |- valid _ _ _ (Bind _ Ret) ] =>
+    eapply valid_equiv;
+    [ apply bind_right_id | ]
+  | [ |- valid _ _ _ (Bind (Bind _ _) _) ] =>
+    eapply valid_equiv;
+    [ apply bind_assoc | ]
+  end.
+
+Ltac monad_simpl := repeat monad_simpl_one.
